case_study/RiscvPmp/Base.v
@@ -1093,6 +1093,123 @@ Module Export RiscvPmpBase <: Base.
 
   End Inhabited.
 
+  Section MemoryModel.
+    Import Bitvector.bv.notations.
+
+    Definition RAM : Type := Addr -> Byte.
+
+    (* Trace of Events *)
+    Inductive EventTy : Set :=
+    | IOWrite
+    | IORead .
+    Record Event : Set :=
+      mkEvent {
+        event_type : EventTy;
+        event_addr : Addr;
+        event_nbbytes : nat;
+        event_contents : bv (event_nbbytes * 8);
+      }.
+    Definition Trace : Set := list Event.
+
+    (* Memory *)
+    Record MemoryType : Type :=
+      mkMem {
+        memory_ram : RAM;
+        memory_trace : Trace;
+        memory_state : State;
+      } .
+    Definition Memory := MemoryType.
+
+    Definition memory_update_ram (μ : Memory) (r : RAM) := mkMem r (memory_trace μ) (memory_state μ).
+    Definition memory_update_trace (μ : Memory) (t : Trace) := mkMem (memory_ram μ) t (memory_state μ).
+    Definition memory_append_trace (μ : Memory) (e : Event) := memory_update_trace μ (cons e (memory_trace μ)).
+    Definition memory_update_state (μ : Memory) (s : State) := mkMem (memory_ram μ) (memory_trace μ) s.
+
+    Fixpoint fun_read_ram (μ : Memory) (data_size : nat) (addr : Val ty_xlenbits) : 
+      Val (ty_bytes data_size) :=
+      match data_size with
+      | O   => bv.zero
+      | S n => bv.app ((memory_ram μ) addr) (fun_read_ram μ n (bv.one + addr))
+      end.
+
+    (* Small test to show that read_ram reads bitvectors in little
+       endian order. *)
+    Goal ∀ μ : Memory,
+      let μ': Memory := memory_update_ram μ (fun a =>
+        if eq_dec a [bv 0x0] then [bv 0xEF] else
+        if eq_dec a [bv 0x1] then [bv 0xBE] else
+        if eq_dec a [bv 0x2] then [bv 0xAD] else
+        if eq_dec a [bv 0x3] then [bv 0xDE] else
+        [bv 0])
+      in fun_read_ram μ' 4 [bv 0] = [bv 0xDEADBEEF].
+    Proof. reflexivity. Qed.
+
+    Definition write_byte (r : RAM) (addr : Val ty_xlenbits) (data : Byte) : RAM :=
+      (fun a => if eq_dec addr a then data else r a).
+
+    Fixpoint fun_write_ram (μ : Memory) (data_size : nat) (addr : Val ty_xlenbits) :
+      Val (ty_bytes data_size) -> Memory :=
+      match data_size as n return (Val (ty_bytes n) → Memory) with
+      | O   => fun _data => μ
+      | S n => fun data : Val (ty_bytes (S n)) =>
+                 let (byte , bytes) := bv.appView 8 (n * 8) data in
+                 let μ' := (memory_update_ram μ (write_byte (memory_ram μ) addr byte)) in
+                 fun_write_ram μ' (bv.one + addr) bytes
+      end.
+    #[global] Arguments fun_write_ram : clear implicits.
+
+    (* Separated into a read and a write function in the sail model *)
+    (* NOTE: we have to check overflow here, because the PMP model does not...*)
+    Definition fun_within_mmio (data_size : nat) (addr : Val ty_xlenbits) : bool :=
+      bool_decide (withinMMIO addr data_size ∧
+      bv.bin addr + N.of_nat data_size < (bv.exp2 xlenbits))%N.
+
+    (* TODO: in principle, restricted bytes don't need a zero-case *)
+    Definition fun_read_mmio (μ : Memory) (data_size : nat) (addr : Val ty_xlenbits) :
+      Memory * Val (ty_bytes data_size) :=
+      match data_size with
+      | O   => (μ , bv.zero)
+      | S n => let (s' , readv) := state_tra_read (memory_state μ) addr data_size in
+               let mmioev := mkEvent IORead addr data_size readv in
+               let μ' := memory_append_trace (memory_update_state μ s') mmioev in
+                (μ' , readv)%type
+      end.
+
+    Definition fun_write_mmio (μ : Memory) (data_size : nat) (addr : Val ty_xlenbits) :
+      Val (ty_bytes data_size) -> Memory :=
+      match data_size as n return (Val (ty_bytes n) → Memory) with
+      | O   => fun _data => μ
+      | S n => fun data : Val (ty_bytes (S n)) =>
+                let s' := state_tra_write (memory_state μ) addr (S n) data in
+                let mmioev := mkEvent IOWrite addr (S n) data in
+                let μ' := memory_append_trace (memory_update_state μ s') mmioev in
+                μ'
+      end.
+
+    Lemma convert_foreign_vector_subrange_conditions {n e b : nat} :
+      IsTrue (0 <=? b)%nat -> IsTrue (b <=? e)%nat -> IsTrue (e <? n)%nat ->
+      IsTrue (b + (e - b + 1) <=? n)%nat.
+    Proof.
+      intros;
+        repeat match goal with
+          | |- IsTrue (?x <=? ?y)%nat =>
+              destruct (Nat.leb_spec x y)
+          | H: IsTrue (?x <=? ?y)%nat |- _ =>
+              destruct (Nat.leb_spec x y)
+          | H: IsTrue (?x <? ?y)%nat |- _ =>
+              destruct (Nat.ltb_spec x y)
+          end;
+        auto;
+        lia.
+    Qed.
+
+    #[program] Definition fun_vector_subrange {n} (data : Val (ty.bvec n)) (e b : nat) {p : IsTrue (0 <=? b)%nat} {q : IsTrue (b <=? e)%nat} {r : IsTrue (e <? n)%nat} : Val (ty.bvec (e - b + 1)) :=
+      @bv.vector_subrange _ b (e - b + 1) _ data.
+    Next Obligation. intros; by apply convert_foreign_vector_subrange_conditions. Defined.
+    #[global] Arguments fun_vector_subrange {n} _ _ _ {_ _ _}.
+
+  End MemoryModel.
+
   Include BaseMixin.
 
 End RiscvPmpBase.
